typeclass/typing/typeclass_typingProofScript.sml
@@ -1,6 +1,7 @@
 open HolKernel Parse boolLib bossLib BasicProvers dep_rewrite;
 open pairTheory arithmeticTheory integerTheory stringTheory optionTheory miscTheory;
 open listTheory alistTheory relationTheory set_relationTheory pred_setTheory;
+open rich_listTheory;
 open pure_cexpTheory pure_configTheory;
 open typeclass_typesTheory typeclass_kindCheckTheory typeclass_typesPropsTheory;
 open pure_tcexpTheory pure_tcexp_typingTheory
@@ -12,5 +13,742 @@ val _ = monadsyntax.enable_monadsyntax();
 val _ = monadsyntax.enable_monad "option";
 
 val _ = new_theory "typeclass_typingProof";
+
+Theorem kind_ok_tdefs_to_tcexp_tdefs:
+  kind_ok (tdefs_to_tcexp_tdefs tds) = kind_ok tds
+Proof
+  simp[lambdify kind_ok_def,tdefs_to_tcexp_tdefs_def] >>
+  rw[FUN_EQ_THM,typedefs_to_cdb_def,oEL_THM,EL_MAP] >>
+  rpt AP_THM_TAC >>
+  rpt AP_TERM_TAC >>
+  rw[FUN_EQ_THM] >>
+  IF_CASES_TAC >>
+  gvs[]
+QED
+
+Theorem typedefs_to_cdb_APPEND:
+  typedefs_to_cdb (tds ++ tds') c =
+  if c < LENGTH tds
+  then typedefs_to_cdb tds c
+  else OPTION_MAP (λtinfo. kind_arrows (FST tinfo) kindType)
+      (LLOOKUP tds' (c - LENGTH tds))
+Proof
+  IF_CASES_TAC >>
+  simp[typedefs_to_cdb_def,oEL_THM,EL_APPEND_EQN] >>
+  Cases_on `0 < LENGTH tds'` >>
+  gvs[]
+QED
+
+Theorem typedefs_to_cdb_SOME_0_LT:
+  typedefs_to_cdb tds c = SOME t ⇒ c < LENGTH tds
+Proof
+  rw[typedefs_to_cdb_def,oEL_THM]
+QED
+
+Theorem kind_ok_tdefs_APPEND:
+  ∀t k. kind_ok tds db t k ⇒
+  kind_ok (tds ++ tds') db t k
+Proof
+  simp[kind_ok_def] >>
+  ho_match_mp_tac kind_wf_ind >>
+  rw[typedefs_to_cdb_APPEND,typedefs_to_cdb_SOME_0_LT] >>
+  metis_tac[]
+QED
+
+Theorem specialises_tdefs_APPEND:
+  specialises tds db s t ⇒
+    specialises (tds ++ tds') db s t
+Proof
+  simp[oneline specialises_def] >>
+  TOP_CASE_TAC >>
+  rw[] >>
+  irule_at (Pos last) EQ_REFL >>
+  drule_at_then (Pos last) irule LIST_REL_mono >>
+  simp[kind_ok_tdefs_APPEND]
+QED
+
+Theorem namespace_ok_IMP_tcexp_namespace_ok:
+  namespace_ok ns ∧
+  ALL_DISTINCT (
+    (MAP implode (SET_TO_LIST reserved_cns)) ++
+    (MAP FST (FST ns)) ++
+    (FLAT (MAP (MAP FST o SND) (SND ns))) ++
+    FLAT (MAP (MAP FST o SND) tds)
+  ) ∧
+  EVERY (λ(ks,td). td ≠ []) tds ∧
+  EVERY (λ(ks,td). EVERY (λ(cn,argtys).
+    EVERY (
+      type_scheme_ok
+        (tdefs_to_tcexp_tdefs (SND ns) ++ tds) ks)
+        argtys) td) tds
+  ⇒
+    tcexp_namespace_ok $ 
+      append_ns (namespace_to_tcexp_namespace ns)
+      ([],tds)
+Proof
+  simp[namespace_to_tcexp_namespace_def,
+    tdefs_to_tcexp_tdefs_def,pair_CASE_def,
+    tcexp_namespace_ok_def,oneline namespace_ok_def,
+    EVERY_MAP,MAP_MAP_o,combinTheory.o_DEF,LAMBDA_PROD,
+    type_scheme_ok_def,
+    lambdify type_ok_def,MAP_FLAT] >>
+  rw[]
+  >- (
+    gvs[ALL_DISTINCT_APPEND,MEM_MAP,MEM_FLAT,
+      GSYM PEXISTS_THM,FORALL_PROD,MEM_FLAT,
+      DISJ_IMP_THM,FORALL_AND_THM,PULL_EXISTS] >>
+    metis_tac[]
+  ) >>
+  gvs[EVERY_MEM,FORALL_PROD] >>
+  rw[] >>
+  irule kind_ok_tdefs_APPEND >>
+  simp[SRULE[tdefs_to_tcexp_tdefs_def] kind_ok_tdefs_to_tcexp_tdefs] >>
+  first_x_assum $ drule_all_then irule
+QED
+
+Theorem class_env_ns_NON_EMPTY:
+  ∀ce' l clcons cl_tds.
+    class_env_to_ns ce cl_to_tyid clcons ce' = SOME cl_tds ∧
+    ce = l ++ ce' ∧
+    LENGTH ce' ≤ LENGTH clcons ⇒
+    EVERY (λ(ks,td). td ≠ []) cl_tds
+Proof
+  Induct >>
+  rw[class_env_to_ns_def] >>
+  Cases_on `clcons` >>
+  gvs[class_env_to_ns_def] >>
+  last_x_assum drule >>
+  rw[] >>
+  gvs[oneline class_to_datatype_def,AllCaseEqs()]
+QED
+
+(* smth like this *)
+Theorem class_env_kind_ok_IMP_type_scheme_ok:
+  class_env_kind_ok tds ce ∧
+  class_env_to_ns ce (ce_to_cl_tyid_map ns_len ce) clcons ce = SOME cl_tds ∧
+  LENGTH ce ≤ LENGTH clcons ⇒
+    EVERY (λ(ks,td). EVERY (λ(cn,argtys).
+      EVERY (
+        type_scheme_ok
+          (SND (namespace_to_tcexp_namespace (exndefs,tds)) ++ cl_tds) ks)
+          argtys) td) cl_tds
+Proof
+  cheat
+QED
+
+Theorem FLOOKUP_ce_to_cl_tyid_map:
+  ALL_DISTINCT (MAP FST ce) ⇒
+  FLOOKUP (ce_to_cl_tyid_map ns_len ce) cl =
+    OPTION_MAP ($+ ns_len) (find_index cl (MAP FST ce) 0)
+Proof
+  simp[ce_to_cl_tyid_map_def,FLOOKUP_FUPDATE_LIST,oneline OPTION_MAP_DEF] >>
+  TOP_CASE_TAC >>
+  gvs[AllCaseEqs(),ALOOKUP_NONE,MAP_REVERSE,MAP_ZIP]
+  >- gvs[MEM_MAP,GSYM find_index_NOT_MEM] >>
+  dxrule_then assume_tac ALOOKUP_MEM >>
+  rpt strip_tac >>
+  gvs[MEM_REVERSE,MEM_ZIP,EL_MAP,EL_GENLIST] >>
+  irule_at (Pos last) ADD_COMM >>
+  drule ALL_DISTINCT_INDEX_OF_EL >>
+  simp[] >>
+  disch_then drule >>
+  simp[EL_MAP,find_index_INDEX_OF]
+QED
+
+Theorem IMP_translate_predicates_SOME:
+  (∀cl. MEM cl l ⇒ ∃k. ce_to_clk ce (FST cl) = SOME k) ∧
+  ALL_DISTINCT (MAP FST ce) ⇒
+  ∃args.
+    translate_predicates (ce_to_cl_tyid_map ns_len ce) l = SOME args
+Proof
+  Induct_on `l` >>
+  rw[translate_predicates_def] >>
+  gvs[FORALL_AND_THM,DISJ_IMP_THM,translate_predicate_def] >>
+  gvs[FLOOKUP_ce_to_cl_tyid_map,ce_to_clk_def] >>
+  metis_tac[ALOOKUP_find_index_SOME]
+QED
+
+Theorem EVERY_pred_type_kind_scheme_ok_IMP_translate_env_SOME:
+  ALL_DISTINCT (MAP FST ce) ⇒
+  ∀env.
+  EVERY (λ(v,scheme).
+    pred_type_kind_scheme_ok (ce_to_clk ce) tds db scheme) env ⇒
+  ∃trans_env. translate_env (ce_to_cl_tyid_map ns_len ce) env =
+    SOME (trans_env: (mlstring # type_kind_scheme) list)
+Proof
+  strip_tac >>
+  Induct >>
+  rw[translate_env_def] >>
+  pairarg_tac >> gvs[translate_env_def] >>
+  PairCases_on `scheme` >>
+  Cases_on `scheme1` >>
+  gvs[pred_type_kind_ok_alt,translate_pred_type_scheme_def,translate_pred_type_def] >>
+  metis_tac[IMP_translate_predicates_SOME]
+QED
+
+Triviality alist_to_fmap_EQ_FUNUPDATE_LIST:
+  alist_to_fmap l = FEMPTY |++ (REVERSE l)
+Proof
+  PURE_REWRITE_TAC[FUPDATE_LIST_EQ_APPEND_REVERSE,]
+QED
+
+Triviality alist_to_fmap_FUNUPDATE_LIST:
+  alist_to_fmap l |++ r = alist_to_fmap (REVERSE r ++ l)
+Proof
+  PURE_REWRITE_TAC[alist_to_fmap_EQ_FUNUPDATE_LIST,
+    REVERSE_APPEND,REVERSE_REVERSE,
+    finite_mapTheory.FUPDATE_LIST_APPEND] >>
+  simp[]
+QED
+
+Theorem IMP_translate_lie_alist_EXISTS_SOME:
+  (∀cl t. (cl,t) ∈ FRANGE (alist_to_fmap (lie_alist:(mlstring # mlstring # type) list)) ⇒
+    ∃k. ce_to_clk ce cl = SOME k) ∧
+  ALL_DISTINCT (MAP FST ce) ∧
+  ALL_DISTINCT (MAP FST lie_alist) ⇒
+  ∃lie_env. translate_lie_alist (ce_to_cl_tyid_map ns_len ce) lie_alist =
+    SOME (lie_env:(mlstring # type_kind_scheme) list)
+Proof
+  Induct_on `lie_alist` >>
+  rw[translate_lie_alist_def] >>
+  PairCases_on `h` >>
+  gvs[translate_lie_alist_def,DISJ_IMP_THM,FORALL_AND_THM,FLOOKUP_ce_to_cl_tyid_map,
+    ce_to_clk_def] >>
+  simp[PULL_EXISTS] >>
+  drule ALOOKUP_find_index_SOME >>
+  rw[] >>
+  gvs[EXISTS_PROD,PULL_EXISTS] >>
+  first_x_assum irule >>
+  rw[] >>
+  last_x_assum irule >>
+  gvs[alist_to_fmap_EQ_FUNUPDATE_LIST,finite_mapTheory.DOMSUB_FUPDATE_LIST,
+    combinTheory.o_DEF] >>
+  `FILTER (λx. h0 ≠ FST x) (REVERSE lie_alist) = REVERSE lie_alist`
+    suffices_by metis_tac[] >>
+  gvs[FILTER_REVERSE,FILTER_EQ_ID,EVERY_MEM,MEM_MAP] >>
+  metis_tac[]
+QED
+
+Theorem type_tcexp_SmartApp_Var:
+  type_tcexp ns db st env (Var x) (Functions arg_tys ret_ty) ∧
+  LIST_REL (λd t. type_tcexp ns db st env (tcexp_of d) t) ds arg_tys ⇒
+  type_tcexp ns db st env (tcexp_of (SmartApp () (Var () x) ds)) ret_ty
+Proof
+  Cases_on `ds` >>
+  rw[] >>
+  gvs[SmartApp_def,cj 1 Functions_def,dest_App_def,tcexp_of_def] >>
+  irule type_tcexp_App >>
+  first_assum $ irule_at (Pos last) >>
+  gvs[LIST_REL_EL_EQN,EL_MAP]
+QED
+
+Theorem type_tcexp_SmartLam:
+  EVERY (type_ok (SND ns) db) arg_tys ∧ LENGTH arg_tys = LENGTH vs ∧
+  type_tcexp ns db st (REVERSE (ZIP (vs,MAP ($, []) arg_tys)) ++ env)
+    (tcexp_of e) ret_ty ⇒
+  type_tcexp ns db st env (tcexp_of $ SmartLam () vs e)
+    (Functions arg_tys ret_ty)
+Proof
+  strip_tac >>
+  Cases_on `vs` >>
+  gvs[SmartLam_def,Functions_def] >>
+  TOP_CASE_TAC
+  >- (
+    gvs[tcexp_of_def] >>
+    irule type_tcexp_Lam >>
+    Cases_on `arg_tys` >>
+    gvs[]
+  ) >>
+  TOP_CASE_TAC >>
+  TOP_CASE_TAC
+  >- (
+    gvs[tcexp_of_def] >>
+    irule type_tcexp_Lam >>
+    Cases_on `arg_tys` >>
+    gvs[]
+  ) >>
+  Cases_on `e` >>
+  gvs[dest_Lam_def,tcexp_of_def] >>
+  qpat_x_assum `type_tcexp _ _ _ _ _ _` $ mp_tac o SRULE[Once type_tcexp_cases] >>
+  rw[] >>
+  simp[GSYM Functions_APPEND] >>
+  irule type_tcexp_Lam >>
+  gvs[REVERSE_ZIP,REVERSE_APPEND,ZIP_APPEND]
+QED
+
+Theorem FST_SND_namespace_to_tcexp_namespace[simp]:
+  SND (namespace_to_tcexp_namespace db) = tdefs_to_tcexp_tdefs (SND db) ∧
+  FST (namespace_to_tcexp_namespace db) = FST db
+Proof
+  simp[namespace_to_tcexp_namespace_def]
+QED
+
+Theorem ALOOKUP_translate_env:
+  ∀trans_env.
+  translate_env cl_to_tyid env = SOME trans_env ⇒
+  ALOOKUP trans_env s = OPTION_BIND
+    (ALOOKUP env s)
+    (translate_pred_type_scheme cl_to_tyid)
+Proof
+  Induct_on `env` >>
+  rw[translate_env_def,FORALL_PROD] >>
+  PairCases_on `h` >>
+  gvs[translate_env_def,ALOOKUP_def] >>
+  IF_CASES_TAC >>
+  gvs[]
+QED
+
+Theorem ALOOKUP_translate_lie_NONE:
+  ∀lie_env.
+  translate_lie_alist cl_to_tyid lie = SOME lie_env ∧
+  ALOOKUP lie s = NONE ⇒
+  ALOOKUP lie_env s = NONE
+Proof
+  Induct_on `lie` >>
+  rw[translate_lie_alist_def] >>
+  PairCases_on `h` >>
+  gvs[translate_lie_alist_def,AllCaseEqs()]
+QED
+
+Theorem ALOOKUP_translate_lie_SOME:
+  ∀lie_env cl t.
+  translate_lie_alist cl_to_tyid lie = SOME lie_env ∧
+  ALOOKUP lie s = SOME (cl,t) ⇒
+  ∃tyid.
+    FLOOKUP cl_to_tyid cl = SOME tyid ∧ 
+    ALOOKUP lie_env s = SOME ([],Cons (UserType tyid) t)
+Proof
+  Induct_on `lie` >>
+  rw[translate_lie_alist_def] >>
+  PairCases_on `h` >>
+  gvs[translate_lie_alist_def,AllCaseEqs()]
+QED
+
+Theorem MEM_FST_translate_lie_alist:
+  ∀lie_env x.
+    translate_lie_alist cl_to_tyid lie_alist = SOME lie_env ∧
+    MEM x lie_env ⇒
+    ∃y z. MEM (FST x,y, z) lie_alist
+Proof
+  Induct_on `lie_alist` >>
+  rw[translate_lie_alist_def] >>
+  PairCases_on `h` >>
+  gvs[translate_lie_alist_def,AllCaseEqs()] >>
+  metis_tac[]
+QED
+
+Theorem ALOOKUP_translate_ie:
+  ∀ie_env.
+  translate_ie_alist cl_to_tyid ie = SOME ie_env ⇒
+  ALOOKUP ie_env s =
+    OPTION_BIND (ALOOKUP ie s) (translate_entailment cl_to_tyid)
+Proof
+  Induct_on `ie` >>
+  rw[translate_ie_alist_def] >>
+  PairCases_on `h` >>
+  gvs[translate_ie_alist_def] >>
+  IF_CASES_TAC >>
+  gvs[]
+QED
+
+Theorem freevars_cexp_SmartApp_Var:
+  freevars_cexp (SmartApp x (Var y v) ds) =
+    {v} ∪ BIGUNION (set (MAP freevars_cexp ds))
+Proof
+  Cases_on `ds` >>
+  gvs[SmartApp_def,freevars_cexp_def,dest_App_def,SF ETA_ss]
+QED
+
+Triviality LIST_REL_pred_tsbust:
+  ∀ps qs. 
+    LIST_REL (λ(c,t) (c',t'). c = c' ∧ tsubst subs t = t')
+      ((cl,t)::ps) ((cl',t')::qs) ⇔
+    cl = cl' ∧
+    tsubst subs t = t' ∧
+    MAP (I ## tsubst subs) ps = qs
+Proof
+  Induct_on `ps`
+  >- (simp[LIST_REL_EL_EQN] >> metis_tac[]) >>
+  gvs[LIST_REL_EL_EQN] >>
+  rw[EQ_IMP_THM] >>
+  ntac 2 (pairarg_tac >> gvs[])
+QED
+
+Theorem specialises_inst_alt:
+  specialises_inst tds (Entail ks ps (cl,t)) (Entail ks' qs (cl',t')) =
+  ∃subs.
+    LIST_REL (kind_ok tds ks') ks subs ∧
+    cl = cl' ∧
+    tsubst subs t = t' ∧
+    MAP (I ## tsubst subs) ps = qs
+Proof
+  simp[specialises_inst_def,LIST_REL_pred_tsbust,SF ETA_ss]
+QED
+
+Theorem translate_predicates_LIST_REL:
+  ∀ps ps'.
+  translate_predicates cl_to_tyid ps = SOME ps' ⇔
+  LIST_REL
+    (λ(cl,t) t'.
+      ∃ut. FLOOKUP cl_to_tyid cl = SOME ut ∧
+        t' = Cons (UserType ut) t)
+    ps ps'
+Proof
+  Induct_on `ps` >>
+  gvs[translate_predicates_def,translate_predicate_def] >>
+  rw[PULL_EXISTS,EQ_IMP_THM] >>
+  pairarg_tac >> gvs[]
+QED
+
+Theorem translate_predicates_subst:
+  ∀ps'.
+    translate_predicates cl_to_tyid (MAP (I ## tsubst subs) l) = SOME ps' ⇒
+    ∃ps. translate_predicates cl_to_tyid l = SOME ps ∧ MAP (tsubst subs) ps = ps'
+Proof
+  Induct_on `l` >>
+  rw[translate_predicates_def,PULL_EXISTS] >>
+  Cases_on `h` >>
+  gvs[translate_predicate_def,subst_db_def]
+QED
+
+Theorem specialises_inst_translate_entailment:
+  specialises_inst tds it (Entail db ps (cl,t)) ∧
+  translate_predicates cl_to_tyid ps = SOME ps' ∧
+  FLOOKUP cl_to_tyid cl = SOME pid ⇒
+  ∃s.
+    translate_entailment cl_to_tyid it = SOME s ∧
+    specialises (tdefs_to_tcexp_tdefs tds ++ cl_tds) db s
+      (Functions ps' (Cons (UserType pid) t))
+Proof
+  simp[oneline translate_entailment_def] >>
+  TOP_CASE_TAC >>
+  simp[oneline specialises_inst_alt,AllCaseEqs(),PULL_EXISTS,
+    translate_predicate_def] >>
+  TOP_CASE_TAC >>  
+  rw[] >>
+  simp[specialises_def,PULL_EXISTS,subst_db_Functions,subst_db_def] >>
+  drule translate_predicates_subst >>
+  rw[] >>
+  simp[] >>
+  irule_at (Pos last) EQ_REFL >>
+  gvs[LIST_REL_EL_EQN] >>
+  rw[] >>
+  first_x_assum $ drule_then assume_tac >>
+  irule kind_ok_tdefs_APPEND >>
+  simp[kind_ok_tdefs_to_tcexp_tdefs]
+QED
+
+Theorem specialises_pred_specialises:
+  specialises_pred (SND ns) db (q,Pred l t') (Pred ps t) ∧
+  translate_predicates (ce_to_cl_tyid_map (LENGTH (SND ns)) ce) ps =
+    SOME ps' ⇒
+  ∃args.
+    translate_predicates (ce_to_cl_tyid_map (LENGTH (SND ns)) ce) l =
+      SOME args ∧
+    specialises (tdefs_to_tcexp_tdefs (SND ns)) db
+      (q,Functions args t') (Functions ps' t)
+Proof
+  rpt strip_tac >>
+  gvs[specialises_pred_def,specialises_def,subst_db_pred_def,
+    subst_db_Functions] >>
+  drule translate_predicates_subst >>
+  rw[] >>
+  simp[] >>
+  irule_at (Pos last) EQ_REFL >>
+  drule_at_then (Pos last) irule $ LIST_REL_mono >>
+  rw[kind_ok_tdefs_to_tcexp_tdefs]
+QED
+
+Theorem construct_dict_type_tcexp:
+  translate_lie_alist cl_to_tyid lie_alist = SOME lie_env ∧
+  translate_ie_alist cl_to_tyid ie_alist = SOME ie_env ∧
+  lie = alist_to_fmap lie_alist ∧
+  ie = alist_to_fmap ie_alist ∧
+  (∀v ent cl t. MEM (v,ent) ie_alist ⇒ ¬MEM (v,cl,t) lie_alist) ∧
+  (∀v ent cl ks ps t. MEM (v,Entail ks ps (cl,t)) ie_alist ⇒
+    ∃pid. FLOOKUP cl_to_tyid cl = SOME pid)
+  ⇒
+  (∀p d. construct_dict tds db ie lie p d ⇒
+    (∀v. v ∈ freevars_cexp d ⇒ ¬MEM v (MAP FST env)) ⇒
+    ∃p'. translate_predicate cl_to_tyid p = SOME p' ∧
+    type_tcexp (exnds,tdefs_to_tcexp_tdefs tds ++ cl_tds) db st
+      (env ++ lie_env ++ ie_env) (tcexp_of d) p') ∧
+  (∀ps ds. construct_dicts tds db ie lie ps ds ⇒
+    (∀d v. MEM d ds ∧ v ∈ freevars_cexp d ⇒ ¬MEM v (MAP FST env)) ⇒
+    ∃ps'. translate_predicates cl_to_tyid ps = SOME ps' ∧ 
+    LIST_REL
+      (λd t.
+        type_tcexp (exnds,tdefs_to_tcexp_tdefs tds ++ cl_tds) db st
+          (env ++ lie_env ++ ie_env) (tcexp_of d) t)
+      ds ps')
+Proof
+  strip_tac >>
+  ho_match_mp_tac construct_dict_ind >>
+  rw[]
+  >- (
+    simp[tcexp_of_def] >>
+    irule_at (Pos last) type_tcexp_Var >>
+    PairCases_on `p` >>
+    simp[ALOOKUP_APPEND] >>
+    reverse $ CASE_TAC
+    >- (
+      drule_then strip_assume_tac ALOOKUP_MEM >>
+      gvs[MEM_MAP]
+    ) >>
+    drule_all ALOOKUP_translate_lie_SOME >>
+    rw[] >>
+    simp[translate_predicate_def,specialises_def]
+  )
+  >- (
+    irule_at (Pos last) type_tcexp_SmartApp_Var >>
+    gvs[freevars_cexp_SmartApp_Var,MEM_MAP,PULL_EXISTS,
+      DISJ_IMP_THM,LEFT_AND_OVER_OR,FORALL_AND_THM] >>
+    qpat_x_assum `_ ⇒
+      ∃ps'. translate_predicates _ _ = SOME _ ∧ LIST_REL _ _ _` mp_tac >>
+    impl_tac >- metis_tac[] >>
+    rw[] >>
+    qpat_assum `LIST_REL _ _ _` $ irule_at Any >>
+    simp[translate_predicate_def,PULL_EXISTS] >>
+    irule_at (Pos hd) type_tcexp_Var >>
+    simp[ALOOKUP_APPEND] >>
+    reverse $ CASE_TAC
+    >- (
+      drule_then strip_assume_tac ALOOKUP_MEM >>
+      gvs[]
+    ) >>
+    reverse $ CASE_TAC
+    >- (
+      imp_res_tac ALOOKUP_MEM >>
+      spose_not_then kall_tac >>
+      qpat_x_assum `∀v ent cl t. MEM (v,ent) ie_alist ⇒ _` drule >>
+      rw[EXISTS_PROD] >>
+      drule_all MEM_FST_translate_lie_alist >>
+      simp[]
+    ) >>
+    drule ALOOKUP_translate_ie >>
+    simp[] >>
+    disch_then kall_tac >>
+    rename1 `specialises_inst _ _ (Entail _ _ p)` >>
+    PairCases_on `p` >>
+    gvs[] >>
+    rename1 `translate_entailment _ it = _` >>
+    Cases_on `it` >>
+    rename1 `Entail _ _ q` >>
+    PairCases_on `q` >>
+    drule_then drule specialises_inst_translate_entailment >>
+    drule_then assume_tac ALOOKUP_MEM >>
+    qpat_x_assum `!v cl ks ps t. _ ⇒ ∃pid. FLOOKUP cl_to_tyid _ = SOME _` drule >>
+    rw[] >>
+    gvs[specialises_inst_alt]
+  )
+  >- (
+    pop_assum mp_tac >>
+    pop_assum mp_tac >>
+    Induct_on `LIST_REL` >>
+    rw[translate_predicates_def,PULL_EXISTS] >>
+    gvs[DISJ_IMP_THM,RIGHT_AND_OVER_OR,FORALL_AND_THM] >>
+    metis_tac[]
+  )
+QED
+
+Theorem translate_lie_alist_APPEND_lie_alist_IMP:
+  ∀vs lie_alist lie_env'.
+    translate_lie_alist cl_to_tyid (vs ++ lie_alist) = SOME lie_env' ⇒
+    ∃vs_env lie_env.
+      translate_lie_alist cl_to_tyid vs = SOME vs_env ∧
+      translate_lie_alist cl_to_tyid lie_alist = SOME lie_env ∧
+      lie_env' = vs_env ++ lie_env
+Proof
+  Induct_on `vs` >>
+  rw[translate_lie_alist_def] >>
+  PairCases_on `h` >>
+  gvs[translate_lie_alist_def,PULL_EXISTS] >>
+  metis_tac[]
+QED
+
+Theorem translate_lie_alist_translate_predicates_SOME:
+  ∀lie_alist lie_env args.
+  translate_lie_alist ce_to_tyid lie_alist = SOME lie_env ∧
+  translate_predicates ce_to_tyid (MAP SND lie_alist) = SOME args ⇒
+  lie_env = ZIP (MAP FST lie_alist, MAP ($, []) args)
+Proof
+  Induct_on `lie_alist` >>
+  rw[translate_lie_alist_def,translate_predicates_def] >>
+  PairCases_on `h` >>
+  gvs[translate_lie_alist_def,translate_predicates_def,translate_predicate_def]
+QED
+
+Theorem translate_predicates_REVERSE:
+  translate_predicates cl_to_tyid (REVERSE ps) = SOME (REVERSE ps') ⇔
+  translate_predicates cl_to_tyid ps = SOME ps'
+Proof
+  simp[translate_predicates_LIST_REL]
+QED
+
+Theorem ALOOKUP_APPEND_EQ:
+  ALOOKUP l x = ALOOKUP l' x ⇒ 
+  ALOOKUP (l ++ r) x = ALOOKUP (l' ++ r) x
+Proof
+  rw[ALOOKUP_APPEND]
+QED
+
+Theorem texp_construct_dict_type_tcexp:
+  class_env_kind_ok (SND ns) ce ∧
+  ALL_DISTINCT (MAP FST ce) ∧
+  class_env_to_ns ce (ce_to_cl_tyid_map (LENGTH $ SND ns) ce)
+    clcons ce = SOME cl_tds ∧
+  LENGTH ce ≤ LENGTH clcons ∧
+  clk = ce_to_clk ce ∧
+  cl_to_tyid = ce_to_cl_tyid_map (LENGTH $ SND ns) ce ∧
+  ie_map = alist_to_fmap ie_alist ∧
+  ie = FRANGE (alist_to_fmap ie_alist) ∧
+  translate_ie_alist cl_to_tyid ie_alist = SOME ie_env
+  ⇒
+  (∀lie db st env e e' pt.
+    pred_type_elaborate_texp ns clk ie lie db st env e e' pt ⇒
+      ∀lie_alist de.
+      lie = FRANGE (alist_to_fmap lie_alist) ∧
+      EVERY (type_ok (SND ns) db) st ∧
+      EVERY (λ(v,scheme). pred_type_kind_scheme_ok clk (SND ns) db scheme) env ∧
+      ALL_DISTINCT (MAP FST lie_alist) ∧
+      (∀cl t. (cl,t) ∈ lie ⇒ ∃k. clk cl = SOME k ∧ kind_ok (SND ns) db k t) ∧
+      pred_texp_construct_dict ns ie_map (alist_to_fmap lie_alist) db
+        (set (MAP FST env)) pt e' de ⇒
+      ∃trans_env lie_env trans_pt.
+        translate_env cl_to_tyid env = SOME trans_env ∧
+        translate_lie_alist cl_to_tyid lie_alist = SOME lie_env ∧
+        translate_pred_type cl_to_tyid pt = SOME trans_pt ∧
+        type_tcexp
+          (append_ns (namespace_to_tcexp_namespace ns) ([],cl_tds))
+          db st
+          (trans_env ++ lie_env ++ ie_env)
+          (tcexp_of de) trans_pt) ∧
+  (∀lie db st env e e' t.
+    type_elaborate_texp ns clk ie lie db st env e e' t ⇒
+      ∀lie_alist de.
+      lie = FRANGE (alist_to_fmap lie_alist) ∧
+      EVERY (type_ok (SND ns) db) st ∧
+      EVERY (λ(v,scheme). pred_type_kind_scheme_ok clk (SND ns) db scheme) env ∧
+      ALL_DISTINCT (MAP FST lie_alist) ∧
+      (∀cl t. (cl,t) ∈ lie ⇒ ∃k. clk cl = SOME k ∧ kind_ok (SND ns) db k t) ∧
+      texp_construct_dict ns ie_map (alist_to_fmap lie_alist) db
+        (set (MAP FST env)) e' de ⇒
+      ∃trans_env lie_env.
+        translate_env cl_to_tyid env = SOME trans_env ∧
+        translate_lie_alist cl_to_tyid lie_alist = SOME lie_env ∧
+        type_tcexp
+          (append_ns (namespace_to_tcexp_namespace ns) ([],cl_tds))
+          db st
+          (trans_env ++ lie_env ++ ie_env)
+          (tcexp_of de) t)
+Proof
+  strip_tac >>
+  ho_match_mp_tac type_elaborate_texp_ind >>
+  rw[]
+  >- (
+    (* Var *)
+    rfs[Once texp_construct_dict_cases] >>
+    drule_all EVERY_pred_type_kind_scheme_ok_IMP_translate_env_SOME >>
+    disch_then $ qspec_then `LENGTH (SND ns)` strip_assume_tac >>
+    first_assum $ irule_at (Pos hd) >>
+    (drule_at_then (Pos last) $ drule_at (Pos last))
+      IMP_translate_lie_alist_EXISTS_SOME >>
+    disch_then $ qspec_then `LENGTH (SND ns)` mp_tac >>
+    impl_tac >- metis_tac[] >>
+    strip_tac >>
+    simp[] >>
+    irule type_tcexp_SmartApp_Var >>
+    irule_at (Pos last) type_tcexp_Var >>
+    drule ALOOKUP_translate_env >>
+    simp[ALOOKUP_APPEND] >>
+    disch_then kall_tac >>
+    simp[translate_pred_type_scheme_def,oneline translate_pred_type_def] >>
+    Cases_on `s` >>
+    simp[] >>
+    CASE_TAC >>
+    simp[AllCaseEqs(),PULL_EXISTS,EXISTS_PROD] >>
+   (drule_then $ drule_then $ drule_at (Pat `construct_dicts _ _ _ _ _ _`)) $
+      cj 2 construct_dict_type_tcexp >>
+    disch_then $ qspecl_then [`st`,`FST ns`,`trans_env`,`cl_tds`] mp_tac >>
+    simp[] >>
+    impl_tac
+    >- cheat >>
+    rw[] >>
+    first_assum $ irule_at (Pos last) >>
+    simp[RIGHT_AND_OVER_OR,EXISTS_OR_THM] >>
+    rpt disj2_tac >>
+    simp[PULL_EXISTS] >>
+    drule_then drule specialises_pred_specialises >>
+    rw[] >>
+    simp[specialises_tdefs_APPEND]
+  )
+  >- (
+    (* Pred *)
+    qpat_x_assum `pred_texp_construct_dict _ _ _ _ _ _ _ _` $ strip_assume_tac o
+      SRULE[Once texp_construct_dict_cases] >>
+    gvs[] >>
+    qpat_x_assum `texp_construct_dict _ _ _ _ _ _ _` $ strip_assume_tac o
+      PURE_REWRITE_RULE[alist_to_fmap_FUNUPDATE_LIST] >>
+    last_x_assum $ drule_at (Pat `texp_construct_dict _ _ _ _ _ _ _`) >>
+    impl_tac
+    >- (
+      simp[MAP_REVERSE,MAP_ZIP,ALL_DISTINCT_APPEND] >>
+      DEP_REWRITE_TAC[finite_mapTheory.FRANGE_FUNION] >>
+      simp[] >>
+      cheat
+    ) >>
+    rw[] >>
+    simp[] >>
+    drule_all_then (qspec_then `LENGTH (SND ns)` strip_assume_tac)
+      EVERY_pred_type_kind_scheme_ok_IMP_translate_env_SOME >>
+    simp[] >>
+    (drule_at_then (Pos last) $ drule_at (Pos last))
+      IMP_translate_lie_alist_EXISTS_SOME >>
+    disch_then $ qspec_then `LENGTH (SND ns)` mp_tac >>
+    impl_tac >- metis_tac[] >>
+    strip_tac >>
+    simp[] >>
+    drule_then strip_assume_tac translate_lie_alist_APPEND_lie_alist_IMP >>
+    simp[translate_pred_type_def,PULL_EXISTS] >>
+    qspecl_then [`LENGTH (SND ns)`,`ps`,`ce`] mp_tac $
+      GEN_ALL IMP_translate_predicates_SOME >>
+    impl_tac
+    >- cheat >>
+    strip_tac >>
+    gvs[] >>
+    irule type_tcexp_SmartLam >>
+    drule $ iffLR translate_predicates_LIST_REL >>
+    gvs[LIST_REL_EL_EQN] >>
+    rw[EVERY_EL]
+    >- (
+      gvs[] >>
+      first_x_assum drule >>
+      pairarg_tac >> rw[] >>
+      gvs[] >>
+      cheat
+      (* class constructor type check *)
+    ) >>
+    drule_then irule type_tcexp_env_extensional >>
+    rpt strip_tac >>
+    imp_res_tac translate_lie_alist_translate_predicates_SOME >>
+    imp_res_tac $ iffRL translate_predicates_REVERSE >>
+    gvs[MAP_ZIP,REVERSE_ZIP,GSYM MAP_REVERSE] >>
+    irule ALOOKUP_APPEND_EQ >>
+    irule ALOOKUP_APPEND_EQ >>
+    simp[ALOOKUP_APPEND,ALOOKUP_ZIP_MAP_SND,oneline OPTION_MAP_DEF] >>
+    CASE_TAC
+    >- (CASE_TAC >> simp[]) >>
+    CASE_TAC >>
+    imp_res_tac ALOOKUP_MEM >>
+    gvs[GSYM REVERSE_ZIP,MEM_REVERSE] >>
+    cheat
+  )
+QED
+
+(*
+Theorem prog_construct_dict_type_tcexp:
+Proof
+QED
+*)
 
 val _ = export_theory();
